AVM/Ecosystem.lean
@@ -1,8 +1,10 @@
 import AVM.Class
 import AVM.Ecosystem.Label
+import AVM.Ecosystem.Member
 
 namespace AVM
 
 /-- Ecosystem is a collection of classes. -/
-structure Ecosystem (label : Ecosystem.Label) where
+structure Ecosystem (label : Ecosystem.Label) : Type 1 where
   classes : (c : label.ClassId) → Class c
+  multiMethods : (f : label.MultiMethodId) → Ecosystem.MultiMethod f
