AVM/Ecosystem/Label.lean
@@ -1,48 +1,60 @@
-import AVM.Class.Label
+import AVM.Ecosystem.Label.Base
 import AVM.Object
 
-namespace AVM.Ecosystem
+namespace AVM.Ecosystem.Label.MultiMethodId
 
-structure Label : Type 1 where
-  name : String
+abbrev Selves' {lab : Ecosystem.Label} (multiId : lab.MultiMethodId) (f : lab.ClassId → Type u) : Type u :=
+  (argName : multiId.ObjectArgNames) → f (lab.MultiMethodObjectArgClass argName)
 
-  ClassId : Type
-  classLabel : ClassId → Class.Label
-  [classesEnum : FinEnum ClassId]
-  [classesRepr : Repr ClassId]
-  [classesBEq : BEq ClassId]
+abbrev Selves {lab : Ecosystem.Label} (multiId : lab.MultiMethodId) : Type := Selves' multiId Object
 
-def Label.classId (l : Label) (clab : Class.Label) : Option l.ClassId :=
-  l.classesEnum.toList.find? (fun b => l.classLabel b == clab)
+def ConsumedToSelves
+  {lab : Ecosystem.Label}
+  {multiId : lab.MultiMethodId}
+  (consumed : List Anoma.Resource)
+  : Option multiId.Selves
+  :=
+  let try consumedVec : Vector Anoma.Resource multiId.numObjectArgs := consumed.toSizedVector
+  let mkConsumedObject (a : multiId.ObjectArgNames) : Option (Object a.classId) := Object.fromResource (consumedVec.get a.ix)
+  @FinEnum.decImageOption'
+    multiId.ObjectArgNames
+    multiId.ObjectArgNamesEnum
+    (fun a => Object a.classId)
+    mkConsumedObject
 
-end AVM.Ecosystem
+def SelvesFromHList
+  {lab : Ecosystem.Label}
+  (multiId : lab.MultiMethodId)
+  (l : HList (multiId.argsClassesVec.toList.map Object))
+  : multiId.Selves := fun arg => by
+  simp [argsClassesVec, List.Vector.toList_ofFn, List.map_ofFn] at l
+  unfold Function.comp at l
+  simp at l
+  let enum := lab.ObjectArgNamesEnum multiId
+  let elem := l.get (by
+                  refine (enum.equiv.toFun arg).cast ?_
+                  simp [List.length_ofFn]
+                  rfl)
+  exact (Eq.mp (by simp) elem)
 
-namespace AVM.Ecosystem.Label
+def SelvesToVector
+  {A : Type u}
+  {lab : Ecosystem.Label}
+  {multiId : lab.MultiMethodId}
+  (selves : multiId.Selves)
+  (f : {arg : multiId.ObjectArgNames} → Object arg.classId → A)
+  : List.Vector A multiId.numObjectArgs
+  := multiId.objectArgNamesVec.map (fun a => f (selves a))
 
-/-- Singleton ecosystem: An ecosystem with a single class, no functions and no intents -/
-def singleton (l : Class.Label) : Ecosystem.Label where
-  name := l.name
+abbrev SelvesIds
+  {lab : Ecosystem.Label}
+  (multiId : lab.MultiMethodId)
+  : Type :=
+  Selves' multiId (fun _ => ObjectId)
 
-  ClassId := PUnit
-  classLabel := fun _ => l
-
-def ClassId.label {lab : Ecosystem.Label} (classId : lab.ClassId) : Class.Label :=
-  lab.classLabel classId
-
-def ClassId.MemberId {lab : Ecosystem.Label} (c : lab.ClassId) := c.label.MemberId
-
-instance ClassId.MemberId.hasTypeRep {lab : Ecosystem.Label} {c : lab.ClassId} : TypeRep c.MemberId := Class.Label.MemberId.hasTypeRep c.label
-
-instance ClassId.MemberId.hasBEq {lab : Ecosystem.Label} {c : lab.ClassId} : BEq c.MemberId := Class.Label.MemberId.hasBEq
-
-instance {lab : Ecosystem.Label} {classId : lab.ClassId}
-  : CoeHead classId.label.ConstructorId classId.MemberId where
-  coe := .constructorId
-
-instance {lab : Ecosystem.Label} {classId : lab.ClassId}
-  : CoeHead classId.label.MethodId classId.MemberId where
-  coe := .methodId
-
-instance {lab : Ecosystem.Label} {classId : lab.ClassId}
-  : CoeHead classId.label.DestructorId classId.MemberId where
-  coe := .destructorId
+def SelvesIdsToVector
+  {lab : Ecosystem.Label}
+  {multiId : lab.MultiMethodId}
+  (selvesIds : multiId.SelvesIds)
+  : List.Vector ObjectId multiId.numObjectArgs :=
+  List.Vector.ofFn (fun i => selvesIds (multiId.ObjectArgNamesEnum.equiv.invFun i))
