AVM/Object.lean
@@ -1,44 +1,68 @@
 import Anoma.Resource
-import AVM.Class.Label
+import AVM.Ecosystem.Label.Base
 
 namespace AVM
 
-structure ObjectData (lab : Class.Label) where
+structure ObjectData {lab : Ecosystem.Label} (c : lab.ClassId) where
   /-- Object quantity, stored in the `quantity` field of the resource. -/
   quantity : Nat
   /-- `privateFields` go into the `value` field of the resource. -/
-  privateFields : lab.PrivateFields.type
+  privateFields : c.label.PrivateFields.type
   deriving BEq
 
-instance ObjectData.inhabited (lab : Class.Label) : Inhabited (ObjectData lab) where
-  default := {quantity := 0, privateFields := lab.privateFieldsInhabited.default}
+instance ObjectData.inhabited {lab : Ecosystem.Label} (c : lab.ClassId) : Inhabited (ObjectData c) where
+  default := {quantity := 0, privateFields := c.label.privateFieldsInhabited.default}
 
-instance ObjectData.hasTypeRep (lab : Class.Label) : TypeRep (ObjectData lab) where
-  rep := Rep.composite "AVM.ObjectData" [Rep.atomic lab.name]
+instance ObjectData.hasTypeRep {lab : Ecosystem.Label} (c : lab.ClassId) : TypeRep (ObjectData c) where
+  rep := Rep.composite "AVM.ObjectData" [Rep.atomic lab.name, Rep.atomic c.label.name]
 
-structure ObjectValue where
-  {label : Class.Label}
+structure SomeObjectData : Type 1 where
+  {label : Ecosystem.Label}
+  {classId : label.ClassId}
+  data : ObjectData classId
+
+instance SomeObjectData.hasTypeRep : TypeRep SomeObjectData where
+  rep := Rep.atomic "AVM.SomeObjectData"
+
+instance SomeObjectData.hasBEq : BEq SomeObjectData where
+  beq a b := a.label === b.label && a.data === b.data
+
+structure ObjectValue : Type 1 where
+  {label : Ecosystem.Label}
+  {classId : label.ClassId}
   uid : ObjectId
-  data : ObjectData label
+  data : ObjectData classId
 
-def ObjectData.toObjectValue {lab : Class.Label} (uid : ObjectId) (data : ObjectData lab) : ObjectValue :=
+instance ObjectValue.hasTypeRep : TypeRep ObjectValue where
+  rep := Rep.atomic "AVM.ObjectValue"
+
+instance ObjectValue.hasBEq : BEq ObjectValue where
+  beq a b := a.label === b.label
+          && a.uid == b.uid
+          && a.data === b.data
+
+def ObjectData.toSomeObjectData {lab : Ecosystem.Label} {c : lab.ClassId} (data : ObjectData c) : SomeObjectData :=
+  ⟨data⟩
+
+def ObjectData.toObjectValue {lab : Ecosystem.Label} {c : lab.ClassId} (uid : ObjectId) (data : ObjectData c) : ObjectValue :=
   ⟨uid, data⟩
 
 /-- Represents a concrete object, translated into a resource. For class
     represetation (object description), see `AVM.Class`. -/
-structure Object.{u} (lab : Class.Label.{u}) : Type u where
+structure Object {lab : Ecosystem.Label} (c : lab.ClassId) : Type where
   /-- Unique object identifier. Stored in the `value` field of the resource. -/
   uid : Anoma.ObjectId
   nonce : Anoma.Nonce
-  data : ObjectData lab
+  data : ObjectData c
   deriving BEq, Inhabited
 
-instance Object.hasTypeRep (lab : Class.Label) : TypeRep (Object lab) where
-  rep := Rep.composite "AVM.Object" [Rep.atomic lab.name]
+instance Object.hasTypeRep {lab : Ecosystem.Label} (c : lab.ClassId) : TypeRep (Object c) where
+  rep := Rep.composite "AVM.Object" [Rep.atomic lab.name, Rep.atomic c.label.name]
 
 structure SomeObject where
-  {label : Class.Label}
-  object : Object label
+  {label : Ecosystem.Label}
+  {classId : label.ClassId}
+  object : Object classId
 
 instance SomeObject.hasTypeRep : TypeRep SomeObject where
   rep := Rep.atomic "AVM.SomeObject"
@@ -46,31 +70,40 @@ instance SomeObject.hasTypeRep : TypeRep SomeObject where
 instance SomeObject.hasBEq : BEq SomeObject where
   beq a b := a.label === b.label && a.object === b.object
 
-def Object.toSomeObject {lab : Class.Label} (object : Object lab) : SomeObject := ⟨object⟩
+def Object.toSomeObject {lab : Ecosystem.Label} {c : lab.ClassId} (object : Object c) : SomeObject := ⟨object⟩
 
-def Object.toObjectValue {lab : Class.Label} (obj : Object lab) : ObjectValue :=
+def Object.toObjectValue {lab : Ecosystem.Label} {c : lab.ClassId} (obj : Object c) : ObjectValue :=
   obj.data.toObjectValue obj.uid
 
+def SomeObject.toObjectValue (object : SomeObject) : ObjectValue where
+  data := object.object.data
+  uid := object.object.uid
+
 structure Object.Resource.Label where
-  /-- The label of the class -/
-  classLabel : Class.Label
+  /-- The label of the ecosystem -/
+  label : Ecosystem.Label
+  /-- The id of the class -/
+  classId : label.ClassId
   /-- The dynamic label is used to put dynamic data into the Resource label -/
-  dynamicLabel : classLabel.DynamicLabel.Label.type
+  dynamicLabel : classId.label.DynamicLabel.Label.type
 
 instance : TypeRep Object.Resource.Label where
   rep := Rep.atomic "Object.Resource.Label"
 
 instance : BEq Object.Resource.Label where
-  beq o1 o2 := o1.classLabel == o2.classLabel && o1.dynamicLabel === o2.dynamicLabel
+  beq o1 o2 :=
+    o1.label == o2.label
+    && o1.classId.label == o2.classId.label
+    && o1.dynamicLabel === o2.dynamicLabel
 
-structure Object.Resource.Value (lab : Class.Label) where
+structure Object.Resource.Value {lab : Ecosystem.Label} (classId : lab.ClassId) where
   uid : Anoma.ObjectId
-  privateFields : lab.PrivateFields.type
+  privateFields : classId.label.PrivateFields.type
 
-instance {lab : Class.Label} : TypeRep (Object.Resource.Value lab) where
-  rep := Rep.composite "Object.Resource.Value" [Rep.atomic lab.name]
+instance {lab : Ecosystem.Label} {classId : lab.ClassId} : TypeRep (Object.Resource.Value classId) where
+  rep := Rep.composite "Object.Resource.Value" [Rep.atomic lab.name, Rep.atomic classId.label.name]
 
-instance {lab : Class.Label} : BEq (Object.Resource.Value lab) where
+instance {lab : Ecosystem.Label} {classId : lab.ClassId} : BEq (Object.Resource.Value classId) where
   beq v1 v2 := v1.uid == v2.uid && v1.privateFields === v2.privateFields
 
 /-- Converts SomeObject to a Resource. -/
@@ -78,41 +111,49 @@ def SomeObject.toResource
   (sobj : SomeObject)
   (ephemeral : Bool)
   : Anoma.Resource :=
-  let lab := sobj.label
-  let obj : Object lab := sobj.object
-  { Val := ⟨Object.Resource.Value lab⟩,
-    Label := ⟨Object.Resource.Label⟩,
-    label := ⟨lab, lab.DynamicLabel.mkDynamicLabel obj.data.privateFields⟩,
-    logicRef := lab.logicRef,
+  let classId := sobj.classId
+  let clab := classId.label
+  let label := sobj.label
+  let obj : Object classId := sobj.object
+  { Label := ⟨Object.Resource.Label⟩,
+    label := { label
+               classId
+               dynamicLabel := clab.DynamicLabel.mkDynamicLabel obj.data.privateFields }
+    logicRef := label.logicRef,
     quantity := obj.data.quantity,
+    Val := ⟨Object.Resource.Value classId⟩,
     value := ⟨obj.uid, obj.data.privateFields⟩,
     ephemeral := ephemeral,
     nonce := obj.nonce,
     nullifierKeyCommitment := default }
 
 /-- Converts Object to a Resource. -/
-def Object.toResource {lab : Class.Label} (obj : Object lab) (ephemeral : Bool) : Anoma.Resource
+def Object.toResource {lab : Ecosystem.Label} {c : lab.ClassId} (obj : Object c) (ephemeral : Bool) : Anoma.Resource
  := obj.toSomeObject.toResource ephemeral
 
 def Object.fromResource
-  {lab : Class.Label}
+  {lab : Ecosystem.Label}
+  {c : lab.ClassId}
   (res : Anoma.Resource)
-  : Option (Object lab) :=
+  : Option (Object c) :=
   let try resLab : Object.Resource.Label := tryCast res.label
-  check (resLab.classLabel == lab)
+  check (resLab.label == lab)
   check (res.logicRef == lab.logicRef)
-  let try value : Object.Resource.Value lab := tryCast res.value
+  let try value : Object.Resource.Value c := tryCast res.value
   some {  uid := value.uid,
           data := ⟨res.quantity, value.privateFields⟩,
           nonce := res.nonce }
 
 def SomeObject.fromResource.{u, v}
   (res : Anoma.Resource.{u, v})
-  : Option SomeObject.{max u v + 1} :=
+  : Option SomeObject :=
   let try resLab : Object.Resource.Label := tryCast res.label
-  let lab : Class.Label := resLab.classLabel
-  let try obj := @Object.fromResource lab res
-  some {label := lab, object := obj}
+  let label : Ecosystem.Label := resLab.label
+  let classId := resLab.classId
+  let try object := @Object.fromResource label classId res
+  some { label
+         classId
+         object }
 
 def Resource.isSomeObject.{u, v} (res : Anoma.Resource.{u, v}) : Bool :=
   Option.isSome (SomeObject.fromResource.{u, v} res)
