Apps/Kudos.lean
@@ -82,28 +82,25 @@ def clab : Class.Label where
   DestructorArgs := fun
     | Destructors.Burn => ⟨PUnit⟩
 
-def label : Ecosystem.Label where
-  name := "KudosEcosystem"
-  ClassId := Classes
-  classLabel := fun
-    | Classes.Kudos => clab
+def label : Ecosystem.Label := Ecosystem.Label.singleton clab
 
-def toObject (c : Kudos) : ObjectData clab where
+def toObject (c : Kudos) : @ObjectData label .unit where
   quantity := c.quantity
   privateFields := { originator := c.originator, owner := c.owner }
 
-def fromObject (o : ObjectData clab) : Kudos :=
+def fromObject (o : @ObjectData label .unit) : Kudos :=
   { owner := o.privateFields.owner
     quantity := o.quantity
     originator := o.privateFields.originator }
 
 instance hasIsObject : IsObject Kudos where
   label := label
-  classId := Classes.Kudos
-  toObject := Kudos.toObject
-  fromObject := Kudos.fromObject
+  classId := .unit
+  isObjectOf :=
+    { toObject := Kudos.toObject
+      fromObject := Kudos.fromObject }
 
-def kudosMint : @Class.Constructor label Classes.Kudos Constructors.Mint := defConstructor
+def kudosMint : @Class.Constructor label .unit Constructors.Mint := defConstructor
   (body := fun (args : MintArgs) => ⟪
     return
       { quantity := args.quantity
@@ -112,14 +109,14 @@ def kudosMint : @Class.Constructor label Classes.Kudos Constructors.Mint := defC
   ⟫)
   (invariant := fun (args : MintArgs) => checkKey args.originator args.key)
 
-def kudosTransfer : @Class.Method label Classes.Kudos Methods.Transfer := defMethod Kudos
+def kudosTransfer : @Class.Method label .unit Methods.Transfer := defMethod Kudos
   (body := fun (self : Kudos) (args : TransferArgs) =>
     ⟪return {self with owner := args.newOwner : Kudos}⟫)
 
-def kudosBurn : @Class.Destructor label Classes.Kudos Destructors.Burn := defDestructor
+def kudosBurn : @Class.Destructor label .unit Destructors.Burn := defDestructor
   (invariant := fun (self : Kudos) (_args : PUnit) => self.originator == self.owner)
 
-def kudosClass : @Class label Classes.Kudos where
+def kudosClass : @Class label .unit where
   constructors := fun
     | Constructors.Mint => kudosMint
   methods := fun
