AVM.lean
@@ -1,7 +1,7 @@
-import AVM.Object
 import AVM.Class
 import AVM.Class.Translation
-import AVM.Task
-import AVM.Task.Translation
+import AVM.Object
 import AVM.Program
 import AVM.Program.Translation
+import AVM.Task
+import AVM.Task.Translation
