AVM/Class/Member.lean
@@ -2,25 +2,25 @@ import AVM.Program
 
 namespace AVM.Class
 
-structure Constructor.{u} {lab : Ecosystem.Label} (cid : lab.ClassId) (constrId : cid.label.ConstructorId) : Type (u + 1) where
+structure Constructor {lab : Ecosystem.Label} (cid : lab.ClassId) (constrId : cid.label.ConstructorId) : Type 1 where
   /-- Constructor call body. -/
-  body : constrId.Args.type → Program lab (ObjectData cid.label)
+  body : constrId.Args.type → Program.{0} lab (ObjectData cid)
   /-- Extra constructor logic. The constructor invariant is combined with
       auto-generated constructor body constraints to create the constructor logic. -/
   invariant : constrId.Args.type → Bool
 
-structure Destructor.{u} {lab : Ecosystem.Label} (cid : lab.ClassId) (destructorId : cid.label.DestructorId) : Type (u + 1) where
+structure Destructor {lab : Ecosystem.Label} (cid : lab.ClassId) (destructorId : cid.label.DestructorId) : Type 1 where
   /-- Destructor call body. -/
-  body : (self : Object cid.label) → destructorId.Args.type → Program lab PUnit
+  body : (self : Object cid) → destructorId.Args.type → Program.{0} lab PUnit
   /-- Extra destructor logic. -/
-  invariant : (self : Object cid.label) → destructorId.Args.type → Bool
+  invariant : (self : Object cid) → destructorId.Args.type → Bool
 
-structure Method {lab : Ecosystem.Label} (cid : lab.ClassId) (methodId : cid.label.MethodId) : Type (u + 1) where
+structure Method {lab : Ecosystem.Label} (cid : lab.ClassId) (methodId : cid.label.MethodId) : Type 1 where
   /-- Method call body. -/
-  body : (self : Object cid.label) → methodId.Args.type → Program lab (Object cid.label)
+  body : (self : Object cid) → methodId.Args.type → Program lab (Object cid)
   /-- Extra method logic. The method invariant is combined with auto-generated
       method body constraints to create the method logic. -/
-  invariant : (self : Object cid.label) → methodId.Args.type → Bool
+  invariant : (self : Object cid) → methodId.Args.type → Bool
 
 /-- A class member is a constructor, a destructor or a method. -/
 inductive Member {lab : Ecosystem.Label} (cid : lab.ClassId) where
