AVM/Class/Translation/Logics.lean
@@ -1,6 +1,7 @@
 import AVM.Class
 import AVM.Message
 import AVM.Logic
+import AVM.Ecosystem
 
 namespace AVM.Class
 
@@ -12,7 +13,7 @@ private def Constructor.Message.logicFun
   (constr : Class.Constructor classId constrId)
   (args : Logic.Args)
   : Bool :=
-  let try msg : Message classId.label := Message.fromResource args.self
+  let try msg : Message lab := Message.fromResource args.self
   let try argsData := SomeType.cast msg.args
   let try vals : (constr.body argsData).params.Product := tryCast msg.vals
   let newObjData := constr.body argsData |>.value vals
@@ -34,12 +35,12 @@ private def Destructor.Message.logicFun
   (destructor : Class.Destructor classId destructorId)
   (args : Logic.Args)
   : Bool :=
-  let try msg : Message classId.label := Message.fromResource args.self
+  let try msg : Message lab := Message.fromResource args.self
   let try argsData := SomeType.cast msg.args
   let consumedResObjs := Logic.selectObjectResources args.consumed
   let createdResObjs := Logic.selectObjectResources args.created
   let! [selfRes] := consumedResObjs
-  let try selfObj : Object classId.label := Object.fromResource selfRes
+  let try selfObj : Object classId := Object.fromResource selfRes
   Logic.checkResourceValues [selfObj.toObjectValue] createdResObjs
     && Logic.checkResourcesPersistent consumedResObjs
     && Logic.checkResourcesEphemeral createdResObjs
@@ -53,16 +54,16 @@ private def Method.Message.logicFun
   (method : Class.Method classId methodId)
   (args : Logic.Args)
   : Bool :=
-  let try msg : Message classId.label := Message.fromResource args.self
+  let try msg : Message lab := Message.fromResource args.self
   let try argsData := SomeType.cast msg.args
   let consumedResObjs := Logic.selectObjectResources args.consumed
   let createdResObjs := Logic.selectObjectResources args.created
   let! [selfRes] := consumedResObjs
-  let try selfObj : Object classId.label := Object.fromResource selfRes
+  let try selfObj : Object classId := Object.fromResource selfRes
   check method.invariant selfObj argsData
   let body := method.body selfObj argsData
   let try vals : body.params.Product := tryCast msg.vals
-  let createdObject : Object classId.label := body |>.value vals
+  let createdObject : Object classId := body |>.value vals
   Logic.checkResourceValues [createdObject.toObjectValue] createdResObjs
     && Logic.checkResourcesPersistent consumedResObjs
     && Logic.checkResourcesPersistent createdResObjs
@@ -70,8 +71,13 @@ private def Method.Message.logicFun
 /-- The class logic checks if all consumed messages in the action correspond to
     class members, the single consumed object is the receiver, and there is
     at least one message. -/
-private def logicFun {lab : Ecosystem.Label} {classId : lab.ClassId} (cl : Class classId) (args : Logic.Args) : Bool :=
-  let try self : Object classId.label := Object.fromResource args.self
+private def logicFun
+  {lab : Ecosystem.Label}
+  {classId : lab.ClassId}
+  (cl : Class classId)
+  (args : Logic.Args)
+  : Bool :=
+  let try self : Object classId := Object.fromResource args.self
   check cl.invariant self args
   match args.status with
   | Created => true
@@ -79,14 +85,15 @@ private def logicFun {lab : Ecosystem.Label} {classId : lab.ClassId} (cl : Class
     let consumedMessageResources : List Anoma.Resource := Logic.selectMessageResources args.consumed
     let nMessages := consumedMessageResources.length
     let! [consumedObjectResource] : List Anoma.Resource := Logic.selectObjectResources args.consumed
-    let try consumedObject : Object classId.label := Object.fromResource consumedObjectResource
+    let try consumedObject : Object classId := Object.fromResource consumedObjectResource
     -- NOTE: consumedObject == self by definition of Logic.Args; we only check
     -- that there are no other consumed objects
     nMessages >= 1
       && nMessages + 1 == (Logic.filterOutDummy args.consumed).length
       && consumedMessageResources.all fun res =>
-        let try msg : Message classId.label := Message.fromResource res
-        consumedObject.uid == msg.recipient
+        let try msg : Message lab := Message.fromResource res
+        let! [recipient] := msg.recipients.toList
+        consumedObject.uid == recipient
 
 def Constructor.Message.logic
   {lab : Ecosystem.Label}
@@ -115,6 +122,95 @@ def Method.Message.logic
   { reference := ⟨s!"AVM.Class.{classId.label.name}.Method.{@repr _ classId.label.methodsRepr methodId}"⟩,
     function := Method.Message.logicFun method }
 
-def logic {lab : Ecosystem.Label} {classId : lab.ClassId} (cl : Class classId) : Anoma.Logic :=
-  { reference := classId.label.logicRef,
-    function := logicFun cl }
+end AVM.Class
+
+namespace AVM.Ecosystem
+
+def MultiMethod.Message.logicFun
+  {lab : Ecosystem.Label}
+  {multiId : lab.MultiMethodId}
+  (method : MultiMethod multiId)
+  (args : Logic.Args)
+  (data : MultiMethodData)
+  : Bool :=
+  let try msg : Message lab := Message.fromResource args.self
+  let try fargs : multiId.Args.type := SomeType.cast msg.args
+  let consumedResObjs := Logic.selectObjectResources args.consumed
+  let createdResObjs := Logic.selectObjectResources args.created
+  let try (argsConsumedSelves, argsConstructedEph, argsDestroyed, .unit) :=
+      consumedResObjs
+      |> Logic.filterOutDummy
+      |>.splitsExact [multiId.numObjectArgs, data.numConstructed, data.numDestroyed]
+  let try argsConsumedObjects : multiId.Selves := Label.MultiMethodId.ConsumedToSelves argsConsumedSelves.toList
+  let prog := method.body argsConsumedObjects fargs
+  method.invariant argsConsumedObjects fargs
+   && let try vals : prog.params.Product := tryCast msg.vals
+      let res : MultiMethodResult multiId := prog |>.value vals
+      let consumedUid (arg : multiId.ObjectArgNames) : Anoma.ObjectId := argsConsumedObjects arg |>.uid
+      let mkObjectValue {classId : lab.ClassId} (arg : multiId.ObjectArgNames) (d : ObjectData classId) : ObjectValue := ⟨consumedUid arg, d⟩
+      let reassembled : List ObjectValue := res.assembled.withOldUidList.map (fun x => mkObjectValue x.arg x.objectData)
+      let destroyedObjects : List ObjectValue := res.destroyed.map (fun x => x.toSomeObject.toObjectValue)
+      let constructedObjects : List ObjectValue := res.constructed
+      let consumedDestroyedObjects : List ObjectValue :=
+        multiId.objectArgNamesVec.toList.filterMap (fun arg =>
+        let argObject := argsConsumedObjects arg
+        match res.argDeconstruction arg with
+        | .Destroyed => argObject |>.data.toObjectValue argObject.uid
+        | .Disassembled => none)
+      let try (argsCreated, argsConstructed, argsDestroyedEph, argsSelvesDestroyedEph, .unit) :=
+        createdResObjs
+        |> Logic.filterOutDummy
+        |>.splitsExact [reassembled.length, data.numConstructed, data.numDestroyed, data.numSelvesDestroyed]
+      Logic.checkResourceValues reassembled argsCreated.toList
+        && Logic.checkResourceValues destroyedObjects argsDestroyed.toList
+        && Logic.checkResourceValues destroyedObjects argsDestroyedEph.toList
+        && Logic.checkResourceValues constructedObjects argsConstructed.toList
+        && Logic.checkResourceValues constructedObjects argsConstructedEph.toList
+        && Logic.checkResourceValues consumedDestroyedObjects argsSelvesDestroyedEph.toList
+        && Logic.checkResourcesPersistent argsConsumedSelves.toList
+        && Logic.checkResourcesPersistent argsDestroyed.toList
+        && Logic.checkResourcesPersistent argsCreated.toList
+        && Logic.checkResourcesPersistent argsConstructed.toList
+        && Logic.checkResourcesEphemeral argsConstructedEph.toList
+        && Logic.checkResourcesEphemeral argsDestroyedEph.toList
+        && Logic.checkResourcesEphemeral argsSelvesDestroyedEph.toList
+
+def MultiMethod.Message.logic
+  {lab : Ecosystem.Label}
+  {multiId : lab.MultiMethodId}
+  (method : MultiMethod multiId)
+  (data : MultiMethodData)
+  : Anoma.Logic :=
+  { reference := ⟨s!"AVM.MultiMethod.{@repr _ lab.multiMethodsRepr multiId}"⟩,
+    function args := MultiMethod.Message.logicFun method args data }
+
+/-- The multiMethod logic checks that all consumed messages in the action correspond
+  to multiMethods and the consumed objects are the receivers. -/
+private def logicFun
+  {lab : Ecosystem.Label}
+  (eco : Ecosystem lab)
+  (memberId : lab.MemberId)
+  (args : Logic.Args)
+  : Bool :=
+  match args.status with
+  | Created => true
+  | Consumed => match memberId with
+    | .classMember (classId := cl) _ => AVM.Class.logicFun (eco.classes cl) args
+    | .multiMethodId multiId =>
+      let consumedMessageResources : List Anoma.Resource := Logic.selectMessageResources args.consumed
+      let nMessages := consumedMessageResources.length
+      let consumedObjectResources : List Anoma.Resource := Logic.selectObjectResources args.consumed
+      let try selves : multiId.Selves := multiId.ConsumedToSelves consumedObjectResources
+      nMessages > 0
+        && nMessages + multiId.numObjectArgs == (Logic.filterOutDummy args.consumed).length
+        && consumedMessageResources.all fun res =>
+          let try msg : Message lab := Message.fromResource res
+          Label.MultiMethodId.SelvesToVector selves (fun o => o.uid) ≍? msg.recipients
+
+def logic
+  {lab : Ecosystem.Label}
+  (eco : Ecosystem lab)
+  (memberId : lab.MemberId)
+  : Anoma.Logic :=
+  { reference := lab.logicRef,
+    function := logicFun eco memberId }
