AVM/Ecosystem/Data.lean
@@ -1,0 +1,28 @@
+import AVM.Ecosystem.Label
+
+namespace AVM
+
+structure MultiMethodData : Type where
+  numConstructed : Nat
+  numDestroyed : Nat
+  numSelvesDestroyed : Nat
+  numReassembledNewUid : Nat
+  numReassembledOldUid : Nat
+  deriving BEq
+
+instance Nonce.hasTypeRep : TypeRep MultiMethodData where
+  rep := Rep.atomic "AVM.MultiMethodData"
+
+structure MultiMethodRandoms (d : MultiMethodData) where
+  destroyedEphRands : List.Vector Nat d.numDestroyed
+  /-- The nonce is also used for uid -/
+  constructedNonces : List.Vector Anoma.Nonce d.numConstructed
+  constructedRands : List.Vector Nat d.numConstructed
+  reassembledNewUidRands : List.Vector Nat d.numReassembledNewUid
+  reassembledNewUidNonces : List.Vector Anoma.Nonce d.numReassembledNewUid
+  reassembledOldUidRands : List.Vector Nat d.numReassembledOldUid
+  selvesDestroyedEphRands : List.Vector Nat d.numSelvesDestroyed
+
+def Ecosystem.Label.MemberId.Data {lab : Ecosystem.Label} : lab.MemberId → Type
+  | .multiMethodId _ => MultiMethodData
+  | _ => Unit
