AVM/Ecosystem/Label/Base.lean
@@ -1,0 +1,147 @@
+import AVM.Class.Label
+
+namespace AVM.Ecosystem
+
+structure Label : Type 1 where
+  name : String
+
+  ClassId : Type
+  classLabel : ClassId → Class.Label
+  [classesEnum : FinEnum ClassId]
+  [classesRepr : Repr ClassId]
+  [classesBEq : BEq ClassId]
+
+  MultiMethodId : Type := Empty
+  /-- Type of multiMethod arguments excluding `self` arguments. -/
+  MultiMethodArgs : MultiMethodId → SomeType := fun _ => ⟨PUnit⟩
+  /-- Names of `self` arguments for a given multiMethod. -/
+  MultiMethodObjectArgNames : MultiMethodId → Type := fun _ => PUnit
+  /-- Class identifiers for `self` arguments. -/
+  MultiMethodObjectArgClass : {f : MultiMethodId} → MultiMethodObjectArgNames f → ClassId
+  [ObjectArgNamesEnum (f : MultiMethodId) : FinEnum (MultiMethodObjectArgNames f)]
+  [ObjectArgNamesBEq (f : MultiMethodId) : BEq (MultiMethodObjectArgNames f)]
+  [multiMethodsFinite : FinEnum MultiMethodId]
+  [multiMethodsRepr : Repr MultiMethodId]
+  [multiMethodsBEq : BEq MultiMethodId]
+
+instance Label.hasTypeRep : TypeRep Label where
+  rep := Rep.atomic "AVM.Ecosystem.Label"
+
+def Label.classId (l : Label) (clab : Class.Label) : Option l.ClassId :=
+  l.classesEnum.toList.find? (fun b => l.classLabel b == clab)
+
+instance hasBEq : BEq Label where
+  beq a b := a.name == b.name
+
+end AVM.Ecosystem
+
+def Fin.classId
+  {lab : AVM.Ecosystem.Label}
+  {multiId : lab.MultiMethodId}
+  (arg : Fin (lab.ObjectArgNamesEnum multiId).card)
+  : lab.ClassId := lab.MultiMethodObjectArgClass ((lab.ObjectArgNamesEnum multiId).equiv.invFun arg)
+
+namespace AVM.Ecosystem.Label
+
+def logicRef (lab : Label) : Anoma.LogicRef :=
+  ⟨"logic-of-ecosystem-" ++ lab.name⟩
+
+/-- Singleton ecosystem: An ecosystem with a single class, no multiMethods and no intents -/
+def singleton (l : Class.Label) : Ecosystem.Label where
+  name := l.name
+
+  ClassId := PUnit
+  classLabel := fun _ => l
+
+  MultiMethodObjectArgClass {f : Empty} := f.elim
+
+def dummy : Label := singleton Class.Label.dummy
+
+def instInhabited : Inhabited Ecosystem.Label where
+  default := dummy
+
+def MultiMethodObjectArgNames.classId
+  {lab : Ecosystem.Label}
+  {multiId : lab.MultiMethodId}
+  (arg : lab.MultiMethodObjectArgNames multiId)
+  : lab.ClassId := lab.MultiMethodObjectArgClass arg
+
+namespace ClassId
+
+def label {lab : Ecosystem.Label} (classId : lab.ClassId) : Class.Label :=
+  lab.classLabel classId
+
+def MemberId {lab : Ecosystem.Label} (c : lab.ClassId) := c.label.MemberId
+
+instance MemberId.hasTypeRep {lab : Ecosystem.Label} {c : lab.ClassId} : TypeRep c.MemberId := Class.Label.MemberId.hasTypeRep c.label
+
+instance MemberId.hasBEq {lab : Ecosystem.Label} {c : lab.ClassId} : BEq c.MemberId := Class.Label.MemberId.hasBEq
+
+end ClassId
+
+instance {lab : Ecosystem.Label} {classId : lab.ClassId}
+  : CoeHead classId.label.ConstructorId classId.MemberId where
+  coe := .constructorId
+
+instance {lab : Ecosystem.Label} {classId : lab.ClassId}
+  : CoeHead classId.label.MethodId classId.MemberId where
+  coe := .methodId
+
+instance {lab : Ecosystem.Label} {classId : lab.ClassId}
+  : CoeHead classId.label.DestructorId classId.MemberId where
+  coe := .destructorId
+
+namespace MultiMethodId
+
+def Args {lab : Ecosystem.Label} (multiId : lab.MultiMethodId) : SomeType :=
+  lab.MultiMethodArgs multiId
+
+def ObjectArgNames {lab : Ecosystem.Label} (multiId : lab.MultiMethodId) : Type :=
+  lab.MultiMethodObjectArgNames multiId
+
+def ObjectArgNamesEnum {lab : Ecosystem.Label} (multiId : lab.MultiMethodId) : FinEnum (lab.MultiMethodObjectArgNames multiId) := lab.ObjectArgNamesEnum multiId
+
+def numObjectArgs {lab : Ecosystem.Label} {multiId : lab.MultiMethodId} : Nat :=
+  (lab.ObjectArgNamesEnum multiId).card
+
+def objectArgNamesVec {lab : Ecosystem.Label} (multiId : lab.MultiMethodId) : List.Vector multiId.ObjectArgNames multiId.numObjectArgs :=
+  (lab.ObjectArgNamesEnum multiId).toVector
+
+def ObjectArgNames.classId {lab : Ecosystem.Label} {multiId : lab.MultiMethodId} (argName : multiId.ObjectArgNames) : lab.ClassId :=
+  lab.MultiMethodObjectArgClass argName
+
+/-- Returns the index of an object argument -/
+def ObjectArgNames.ix {lab : Ecosystem.Label} {multiId : lab.MultiMethodId} (argName : multiId.ObjectArgNames) : Fin (lab.ObjectArgNamesEnum multiId).card :=
+  (lab.ObjectArgNamesEnum multiId).equiv.toFun argName
+
+def argsClassesVec {lab : Ecosystem.Label} (multiId : lab.MultiMethodId) : List.Vector lab.ClassId multiId.numObjectArgs :=
+  List.Vector.ofFn (fun (a : Fin numObjectArgs) => lab.MultiMethodObjectArgClass
+  ((lab.ObjectArgNamesEnum multiId).equiv.invFun a))
+
+end MultiMethodId
+
+inductive MemberId (lab : Ecosystem.Label) where
+  | multiMethodId (funId : lab.MultiMethodId)
+  | classMember {classId : lab.ClassId} (memId : classId.MemberId)
+
+namespace MemberId
+
+def Args {lab : Ecosystem.Label} (memberId : MemberId lab) : SomeType :=
+  match memberId with
+  | multiMethodId f => lab.MultiMethodArgs f
+  | classMember m => Class.Label.MemberId.Args m
+
+instance hasBEq {lab : Ecosystem.Label} : BEq (Ecosystem.Label.MemberId lab) where
+  beq a b :=
+    match a, b with
+    | multiMethodId c1, multiMethodId c2 => lab.multiMethodsBEq.beq c1 c2
+    | multiMethodId _, _ => false
+    | _, multiMethodId _ => false
+    | classMember c1, classMember c2 => c1 === c2
+
+def numObjectArgs {lab : Ecosystem.Label} (memberId : MemberId lab) : Nat :=
+  match memberId with
+  | multiMethodId f => f.numObjectArgs
+  | classMember _ => 1
+
+end MemberId
