AVM/Ecosystem/Member.lean
@@ -1,0 +1,102 @@
+import AVM.Program
+import AVM.Ecosystem.Label
+import AVM.Ecosystem.Data
+import AVM.Object.Consumed
+
+namespace AVM
+
+inductive DeconstructionKind : Type where
+  /-- Will be consumed and automatically balanced with an ephemeral resource -/
+  | Destroyed
+  /-- Will be consumed. It is the responsibility of the user to balance disassembled objects with assembled objects -/
+  | Disassembled
+  deriving BEq, DecidableEq
+
+structure Assembled
+  {label : Ecosystem.Label}
+  {multiId : label.MultiMethodId}
+  (argDeconstruction : multiId.ObjectArgNames → DeconstructionKind)
+  : Type 1 where
+  /-- It is possible that a disassembled Object's uid is not in any of the created objects. Consider
+      the situation when you want to split an object into two and it is desirable that none of the
+      spawned objects has the uid of the original --/
+  withOldUid : (arg : multiId.ObjectArgNames) → argDeconstruction arg = .Disassembled → Option (ObjectData arg.classId)
+  withNewUid : List SomeObjectData
+
+structure AssembledOldUid
+  {label : Ecosystem.Label}
+  {multiId : label.MultiMethodId}
+  {argDeconstruction : multiId.ObjectArgNames → DeconstructionKind}
+  (a : Assembled argDeconstruction)
+  : Type 1 where
+  arg : multiId.ObjectArgNames
+  objectData : ObjectData arg.classId
+  disassembled : argDeconstruction arg = .Disassembled
+  correct : a.withOldUid arg disassembled = some objectData
+
+def Assembled.withOldUidList
+  {lab : Ecosystem.Label}
+  {multiId : lab.MultiMethodId}
+  {argDeconstruction : multiId.ObjectArgNames → DeconstructionKind}
+  (assembled : Assembled argDeconstruction)
+  : List (AssembledOldUid assembled)
+  := multiId.objectArgNamesVec.toList.filterMap fun arg =>
+    if disassembled : argDeconstruction arg = .Disassembled
+    then match correct : assembled.withOldUid arg disassembled with
+         | none => none
+         | some objectData => some
+            { arg
+              objectData
+              disassembled
+              correct }
+    else none
+
+instance Assembled.instInhabited
+  {lab : Ecosystem.Label}
+  {multiId : lab.MultiMethodId}
+  (argDeconstruction : multiId.ObjectArgNames → DeconstructionKind)
+  : Inhabited (Assembled argDeconstruction) where
+  default :=
+    { withNewUid := []
+      withOldUid := fun _ _ => .none }
+
+structure MultiMethodResult {lab : Ecosystem.Label} (multiId : lab.MultiMethodId) : Type 1 where
+  /-- For each object argument we specify its usage. See `Usage`.
+  Note that if `argUsage arg = .Destroyed`, then the object that corresponds to `arg` should *not* be put in the destroyed list -/
+  argDeconstruction : multiId.ObjectArgNames → DeconstructionKind
+  /-- List of assembled objects. Assembled objects will be created.
+      It is the responsibility of the user to ensure that
+      assembled objects balance with the object arguments that are disassembled -/
+  assembled : Assembled argDeconstruction
+  /-- List of destroyed objects. Destroyed objects will be balanced with automatically generated ephemeral resources -/
+  destroyed : List SomeConsumableObject := []
+  /-- List of constructed objects. Constructed objects will be balanced with automatically generated ephemeral resources -/
+  constructed : List ObjectValue := []
+
+namespace MultiMethodResult
+
+instance instInhabited {lab : Ecosystem.Label} {multiId : lab.MultiMethodId} : Inhabited (MultiMethodResult multiId) where
+  default :=
+    { argDeconstruction := fun _ => .Disassembled
+      assembled := default
+      destroyed := []
+      constructed := [] }
+
+def computeMultiMethodData
+  {lab : Ecosystem.Label}
+  {multiId : lab.MultiMethodId}
+  (res : MultiMethodResult multiId)
+  : MultiMethodData :=
+  { numConstructed := res.constructed.length
+    numDestroyed := res.destroyed.length
+    numSelvesDestroyed := multiId.objectArgNamesVec.toList.countP (fun x => res.argDeconstruction x == .Destroyed)
+    numReassembledNewUid := res.assembled.withNewUid.length
+    numReassembledOldUid := res.assembled.withOldUidList.length }
+
+end MultiMethodResult
+
+structure Ecosystem.MultiMethod {lab : Ecosystem.Label} (multiId : lab.MultiMethodId) : Type 1 where
+  /-- Computes the result of a multiMethod call. See `MultiMethodResult`. -/
+  body (selves : multiId.Selves) (args : multiId.Args.type) : Program.{1} lab (MultiMethodResult multiId)
+  /-- Extra multiMethod logic. -/
+  invariant (selves : multiId.Selves) (args : multiId.Args.type) : Bool
