AVM/Tasks.lean
@@ -7,7 +7,7 @@ namespace AVM
   structure of AVM programs than a single `Task`. `AVM.Program` is compiled to
   `Tasks` which are then composed into a single `Task`. The composition of
   `Tasks` collects and lifts out the parameters of all subtasks. -/
-inductive Tasks (α : Type u) where
+inductive Tasks (α : Type u) : Type (max u 1) where
   /-- Execute a subtask and continue. The `rest` continuation receives the
     unadjusted parameter values. -/
   | task (task : Task) (rest : task.params.Product → Tasks α) : Tasks α
@@ -15,17 +15,98 @@ inductive Tasks (α : Type u) where
     unadjusted original object value and is supposed to adjust it by the
     modifications to that object that occurred from the start of the program up
     to the fetch. -/
-  | fetch {classLabel : Class.Label} (objId : ObjectId) (rest : Object classLabel → Tasks α) : Tasks α
+  | fetch {label : Ecosystem.Label} {classId : label.ClassId} (objId : ObjectId) (rest : Object classId → Tasks α) : Tasks α
   | rand (rest : Nat → Tasks α) : Tasks α
   | result (value : α) : Tasks α
   deriving Inhabited
+
+structure ActionData : Type 1 where
+  consumed : List SomeConsumableObject
+  created : List CreatedObject
+  ensureUnique : List Anoma.Nonce := []
+
+namespace Tasks
+
+def rands
+  {α : Type u}
+  (n : Nat)
+  (rest : List.Vector Nat n → Tasks α)
+  : Tasks α := match n with
+  | 0 => rest (List.Vector.ofFn nofun)
+  | .succ m => rands m fun v => .rand fun r => rest (v.cons r)
+
+def fetchMany
+  {α : Type u}
+  {label : Ecosystem.Label}
+  (params : List (label.ClassId × ObjectId))
+  (rest : Pi (params.map (fun param => Object param.1)) (Tasks α))
+  : Tasks α :=
+  match params with
+  | [] => rest.down
+  | i :: is => .fetch i.2 (fun o => fetchMany is (rest o))
+
+def fetchManyHList
+  {α : Type u}
+  {label : Ecosystem.Label}
+  (params : List (label.ClassId × ObjectId))
+  (rest : HList (params.map (fun param => Object param.1)) → Tasks α)
+  : Tasks α := fetchMany params (HList.toPi rest)
+
+def fetchSelves
+  {α : Type u}
+  {lab : Ecosystem.Label}
+  {multiId : lab.MultiMethodId}
+  (selvesIds : multiId.SelvesIds)
+  (rest : multiId.Selves → Tasks α)
+  : Tasks α :=
+    fetchManyHList
+      (multiId.objectArgNamesVec.toList.map (fun arg =>
+                                     { snd := selvesIds arg
+                                       fst := arg.classId}))
+      (fun h => rest ( multiId.SelvesFromHList (by
+        simp at h
+        unfold Function.comp at h
+        simp at h
+        refine (Eq.mp ?_ h)
+        congr 1
+        unfold Ecosystem.Label.MultiMethodId.argsClassesVec
+               Ecosystem.Label.MultiMethodId.objectArgNamesVec
+        simp
+        unfold Function.comp FinEnum.toVector
+        simp
+        unfold Function.comp
+        apply funext
+        intro x
+        congr 1)))
+
+def genMultiMethodRandoms
+  {α : Type u}
+  (d : MultiMethodData)
+  (rest : MultiMethodRandoms d → Tasks α)
+  : Tasks α :=
+   rands _ fun constructedNoncesNats =>
+   rands _ fun constructedRands =>
+   rands _ fun reassembledNewUidRands =>
+   rands _ fun reassembledOldUidRands =>
+   rands _ fun selvesDestroyedEphRands =>
+   rands _ fun destroyedEphRands =>
+   rands _ fun reassembledNewUidNonces =>
+   {
+     destroyedEphRands
+     constructedNonces := constructedNoncesNats.map Anoma.Nonce.mk
+     reassembledNewUidNonces := reassembledNewUidNonces.map Anoma.Nonce.mk
+     constructedRands
+     reassembledNewUidRands
+     reassembledOldUidRands
+     selvesDestroyedEphRands
+    } |> rest
 
 /-- `Tasks.params` includes the parameters of the sub-tasks, in contrast to
   `Program.params` which doesn't include the parameters of the sub-programs. In
   general, values in `tasks.params.Product` are assumed to be unadjusted (see
   `Program.Parameters.Product`), in contrast to values in `prog.params.Product`
   which are assumed to be adjusted. -/
-def Tasks.params {α} (tasks : Tasks α) : Program.Parameters :=
+def params {α} (tasks : Tasks α) : Program.Parameters :=
   match tasks with
   | .task t rest => (t.params.append (fun vals => (rest vals).params))
   | .fetch p rest => .fetch p (fun obj => (rest obj).params)
@@ -36,7 +117,7 @@ def Tasks.params {α} (tasks : Tasks α) : Program.Parameters :=
   `Program.Parameters.Product`): the object values as fetched from Anoma at the
   start of program execution, i.e., they are not adjusted by subsequent
   modifications to these objects in the program. -/
-def Tasks.value {α} (tasks : Tasks α) (vals : tasks.params.Product) : α :=
+def value {α} (tasks : Tasks α) (vals : tasks.params.Product) : α :=
   match tasks with
   | .task _ rest =>
     let ⟨vals1, vals2⟩ := vals.split
@@ -49,17 +130,17 @@ def Tasks.value {α} (tasks : Tasks α) (vals : tasks.params.Product) : α :=
     Tasks.value (rest r) vals'
   | .result v => v
 
-def Tasks.map' {α β} (tasks : Tasks α) (f : tasks.params.Product → α → β) : Tasks β :=
+def map' {α β} (tasks : Tasks α) (f : tasks.params.Product → α → β) : Tasks β :=
   match tasks with
   | .task t rest => .task t (fun vals => map' (rest vals) (fun vals' => f (vals.append vals')))
   | .fetch p rest => .fetch p (fun obj => map' (rest obj) (fun vals' => f ⟨obj, vals'⟩))
   | .rand rest => .rand (fun r => map' (rest r) (fun vals' => f ⟨r, vals'⟩))
   | .result v => .result (f () v)
 
-def Tasks.map {α β} (tasks : Tasks α) (f : α → β) : Tasks β :=
+def map {α β} (tasks : Tasks α) (f : α → β) : Tasks β :=
   tasks.map' (fun _ a => f a)
 
-def Tasks.coerce {α β} {tasks : Tasks α} {f : tasks.params.Product → α → β} (vals : (tasks.map' f).params.Product) : tasks.params.Product :=
+def coerce {α β} {tasks : Tasks α} {f : tasks.params.Product → α → β} (vals : (tasks.map' f).params.Product) : tasks.params.Product :=
   match tasks with
   | .task _ _ =>
     let ⟨vals1, vals2⟩ := vals.split
@@ -72,10 +153,10 @@ def Tasks.coerce {α β} {tasks : Tasks α} {f : tasks.params.Product → α →
     ⟨r, coerce vals'⟩
   | .result _ => vals
 
-def TasksWithAction := Tasks (Rand (Option (Anoma.Action × Anoma.DeltaWitness)))
+def WithAction := Tasks (Rand (Option (Anoma.Action × Anoma.DeltaWitness)))
 
-def Tasks.composeActions
-  (tasks : TasksWithAction)
+def composeActions
+  (tasks : WithAction)
   (vals : tasks.params.Product)
   : Rand (Option Task.Actions) :=
   match tasks with
@@ -96,7 +177,7 @@ def Tasks.composeActions
     let ⟨r, vals'⟩ := vals
     composeActions (rest r) vals'
 
-def Tasks.composeMessages {α} (tasks : Tasks α) (vals : tasks.params.Product) : List SomeMessage :=
+def composeMessages {α} (tasks : Tasks α) (vals : tasks.params.Product) : List SomeMessage :=
   match tasks with
   | .result _ => []
   | .task ta tasks' =>
@@ -110,31 +191,36 @@ def Tasks.composeMessages {α} (tasks : Tasks α) (vals : tasks.params.Product) 
     let ⟨r, vals'⟩ := vals
     composeMessages (rest r) vals'
 
-def Tasks.composeWithAction
-  (tasks : TasksWithAction)
+def composeWithAction
+  (tasks : WithAction)
   (msg : tasks.params.Product → Option SomeMessage)
   : Task :=
   { params := tasks.params,
     message := msg,
     actions := composeActions tasks }
 
-def Tasks.composeWithMessage
+def composeWithMessage
   {α}
   (tasks : Tasks α)
   (msg : α → SomeMessage)
-  (objects : α → List SomeConsumableObject × List CreatedObject)
+  (mkActionData : α → ActionData)
   : Task :=
   let mkAction (vals : tasks.params.Product) (a : α)
     : Rand (Option (Anoma.Action × Anoma.DeltaWitness)) :=
-    let (consumedObjs, createdObjects) := objects a
-    let try consumedObjects := consumedObjs.map (·.consume) |>.getSome
+    let actionData := mkActionData a
+    let try consumedObjects := actionData.consumed.map (·.consume) |>.getSome
     let createdMessages := composeMessages tasks vals
-    Action.create consumedObjects createdObjects [msg a] createdMessages
+    Action.create consumedObjects actionData.created actionData.ensureUnique [msg a] createdMessages
   Tasks.composeWithAction (tasks.map' mkAction) (fun vals => some (msg (tasks.value (coerce vals))))
 
-def Tasks.compose (tasks : Tasks Unit) : Task :=
+def void {α : Type u} (tasks : Tasks α) : Tasks Unit :=
+  tasks.map (fun _ => .unit)
+
+def compose (tasks : Tasks Unit) : Task :=
   let mkAction (vals : tasks.params.Product) (_ : Unit)
     : Rand (Option (Anoma.Action × Anoma.DeltaWitness)) :=
     let createdMessages := tasks.composeMessages vals
-    Action.create [] [] [] createdMessages
+    Action.create [] [] [] [] createdMessages
   Tasks.composeWithAction (tasks.map' mkAction) (fun _ => none)
+
+end Tasks
