Prelude/ULift.lean
@@ -1,0 +1,4 @@
+namespace ULift
+
+instance instInhabited {α : Type u} [Inhabited α] : Inhabited (ULift α) where
+  default := ULift.up default
